MOC Tutorial Week3
===

7.
---



8.
---

***Well-typed***

```Haskell
f :: Num a => b -> a
```

9.
---

No answer required.

10.
---

### a)


| $ P $ | $ Q $ | $ \neg P \implies Q $ | $ P \implies \neg Q $ |
|:------|:------|:----------------------|:----------------------|
| 0     | 0     | 0                     | 1                     |
| 0     | 1     | 1                     | 1                     |
| 1     | 0     | 1                     | 1                     |
| 1     | 1     | 1                     | 0                     |

### b)

| $ P $ | $ Q $ | $ \neg P \implies Q $ | $ Q \implies \neg P $ |
|:------|:------|:----------------------|:----------------------|
| 0     | 0     | 0                     | 1                     |
| 0     | 1     | 1                     | 1                     |
| 1     | 0     | 1                     | 1                     |
| 1     | 1     | 1                     | 0                     |

### c)

| $ P $   | $ Q $   | $ \neg P \implies Q $   | $ \neg Q \implies P $   |
| :------ | :------ | :---------------------- | :---------------------- |
| 0       | 0       | 0                       | 0                        |
| 0       | 1       | 1                       | 1                        |
| 1       | 0       | 1                       | 1                        |
| 1       | 1       | 1                       | 1                        |

### d)

| $ P $ | $ Q $ | $ R $ | $ P \implies (Q \implies R) $ | $ Q \implies (P \implies R) $ |
|-------|-------|-------|-------------------------------|-------------------------------|
|     0 |     0 |     0 |                             1 |                             1 |
|     0 |     1 |     0 |                             1 |                             1 |
|     1 |     0 |     0 |                             1 |                             1 |
|     1 |     1 |     0 |                             0 |                             0 |
|     0 |     0 |     1 |                             1 |                             1 |
|     0 |     1 |     1 |                             1 |                             1 |
|     1 |     0 |     1 |                             1 |                             1 |
|     1 |     1 |     1 |                             1 |                             1 |

### e)

| $ P $ | $ Q $ | $ R $ | $ P \implies (Q \implies R) $ | $ (P \implies Q) \implies R $ |
|-------|-------|-------|-------------------------------|-------------------------------|
|     0 |     0 |     0 |                             1 |                             0 |
|     0 |     1 |     0 |                             1 |                             0 |
|     1 |     0 |     0 |                             1 |                             1 |
|     1 |     1 |     0 |                             0 |                             0 |
|     0 |     0 |     1 |                             1 |                             1 |
|     0 |     1 |     1 |                             1 |                             1 |
|     1 |     0 |     1 |                             1 |                             1 |
|     1 |     1 |     1 |                             1 |                             1 |

### f)

| $ P $   | $ Q $   | $ (P \implies Q) \implies P $ | $ P $                   |
| :------ | :------ | :----------------------       | :---------------------- |
| 0       | 0       | 0                             | 0                       |
| 0       | 1       | 0                             | 0                       |
| 1       | 0       | 1                             | 1                       |
| 1       | 1       | 1                             | 1                       |

### g)

| $ P $ | $ Q $ | $ R $ | $ P \lor Q \implies R $ | $ (P \implies R) \land (Q \implies R) $ |
|-------|-------|-------|-------------------------|-----------------------------------------|
|     0 |     0 |     0 |                       1 |                                       1 |
|     0 |     1 |     0 |                       0 |                                       0 |
|     1 |     0 |     0 |                       0 |                                       0 |
|     1 |     1 |     0 |                       0 |                                       0 |
|     0 |     0 |     1 |                       1 |                                       1 |
|     0 |     1 |     1 |                       1 |                                       1 |
|     1 |     0 |     1 |                       1 |                                       1 |
|     1 |     1 |     1 |                       1 |                                       1 |

11.
---

For $ \iff $

| $ P $ | $ Q $ | $ P \iff Q $ |
|-------|-------|--------------|
|     0 |     0 |            1 |
|     0 |     1 |            0 |
|     1 |     0 |            0 |
|     1 |     1 |            1 |


| $ P $ | $ Q $ | $ P \iff (P \land Q) $ |
|-------|-------|------------------------|
|     0 |     0 |                      1 |
|     0 |     1 |                      1 |
|     1 |     0 |                      0 |
|     1 |     1 |                      1 |

Ans: $ P \implies Q $

12.
---

$$\begin{eqnarray} 
(P \oplus Q) \oplus Q \nonumber \\
\iff P \oplus (Q \oplus Q) \nonumber \\
\iff P \oplus 0 \nonumber \\
\iff P
\end{eqnarray}$$

13.
---

| $ P $ | $ Q $ | $ P \iff Q $ | $ \neg P \iff \neg Q $ |
|-------|-------|--------------|------------------------|
|     0 |     0 |            1 |                      1 |
|     0 |     1 |            0 |                      0 |
|     1 |     0 |            0 |                      0 |
|     1 |     1 |            1 |                      1 |

Shown that $ P \iff Q \quad \equiv \quad \neg P \iff \neg Q $

14.
---

